coq-osiris/theories/semantics/step.v
@@ -200,7 +200,7 @@ Definition step_install_1 σ l (deep : bool) η bs l' :=
   if deep then
     <[l' := K (λ o, Handle (stop CResume (l, o)) (λ o, @bind _ val _
                                                          (wrap_outcome η bs o)
-                                                         (λ o, deep_match η o bs)))]> σ
+                                                         (λ o, eval_branches η o bs)))]> σ
   else
     <[l' := K (λ o, Handle (stop CResume (l, o)) (λ o, shallow_match η o bs bs))]> σ.
 
@@ -690,7 +690,7 @@ Lemma invert_step_install_deep {A E} σ σ' l η bs k m' :
     σ' = <[ l' := K (λ o, Handle (stop CResume (l, o))
                             (λ o, bind
                                     (wrap_outcome η bs o)
-                                    (λ o, deep_match η o bs))) ]> σ ∧
+                                    (λ o, eval_branches η o bs))) ]> σ ∧
   m' = continue k l'.
 Proof.
   intros Hstep. destruct_step.
